



Lo stato iniziale è  $q_0$

$$\begin{aligned} \delta_H = E(\{q_0\}, a) &= \delta_H(E(\{q_0\}, a)) = \{q_1\} \\ \delta_H = E(\{q_0\}, b) &= \delta_H(E(\{q_0\}, b)) = \{q_2\} \\ \delta_H = E(\{q_1\}, a) &= \delta_H(E(\{q_1\}, a)) = \{q_1, q_2\} \\ \delta_H = E(\{q_1\}, b) &= \delta_H(E(\{q_1\}, b)) = \{q_1\} \\ \delta_H = E(\{q_2\}, a) &= \delta_H(E(\{q_2\}, a)) \cup \delta_H(E(\{q_2\}, a)) = \{q_1, q_2\} \cup \emptyset = \{q_1, q_2\} \\ \delta_H = E(\{q_2\}, b) &= \delta_H(E(\{q_2\}, b)) \cup \delta_H(E(\{q_2\}, b)) = \{q_1\} \cup \{q_2\} = \{q_1, q_2\} \\ \delta_H = E(\{q_3\}, a) &= \delta_H(E(\{q_3\}, a)) = \{q_3\} \\ \delta_H = E(\{q_3\}, b) &= \delta_H(E(\{q_3\}, b)) = \{q_3, q_4\} \\ \delta_H = E(\{q_4\}, a) &= \delta_H(E(\{q_4\}, a)) \cup \delta_H(E(\{q_4\}, a)) = \{q_3\} \cup \emptyset = \{q_3\} \\ \delta_H = E(\{q_4\}, b) &= \delta_H(E(\{q_4\}, b)) \cup \delta_H(E(\{q_4\}, b)) = \{q_3, q_4\} \cup \emptyset = \{q_3, q_4\} \end{aligned}$$

